Finished the first demo.

demo/Verif_treeread.v
@@ -1,8 +1,8 @@
-(** * Demo: Traversing Imperative Structures *) 
+(** * Demo: Traversing Imperative Structures *)
 
 (** A brief demo on how to use the CertiGraph library.
 
-Consider the following C program: 
+Consider the following C program:
 
 <<
 #include <stdlib.h>
@@ -22,7 +22,7 @@ unsigned int sum (struct tree *t) {
 }
 >>
 
-*) 
+*)
 
 Require Import VST.floyd.proofauto.
 Require Import VST.msl.iter_sepcon.
@@ -33,15 +33,15 @@ Definition Vprog : varspecs. mk_varspecs prog. Defined.
 
 Definition t_struct_tree := Tstruct _tree noattr.
 
-(** The Coq representation of a tree is a nested tuple of three values. *) 
-Compute (reptype t_struct_tree). 
+(** The Coq representation of a tree is a nested tuple of three values. *)
+Compute (reptype t_struct_tree).
 
-(** ** The Functional Model 
+(** ** The Functional Model
 
 Our functional model contains
 -  a data structure of trees, where a tree is either a leaf [E] or a binary node [T n tl tr] with a label [n], left subtree [tl], and right subtree [tr]
 - the function [sum] which adds up all labels in a tree.
- *) 
+ *)
 Inductive tree : Type :=
  | E: tree
  | T: int -> tree -> tree -> tree.
@@ -52,15 +52,14 @@ Fixpoint sum (t : tree) : int :=
   | T n tl tr => Int.add n (Int.add (sum tl) (sum tr))
   end.
 
-
 (** ** Simplified model
 
   We start with a simplified model which highlights the general localization tactics.
-*) 
+*)
 
 Module SimplifiedModel.
 
-(** In this simplified model, a graph is a list of the addresses and representations of trees. *) 
+(** In this simplified model, a graph is a list of the addresses and representations of trees. *)
 Definition graph := list (val * reptype t_struct_tree).
 
 (** A graph representation separates all trees. *)
@@ -69,9 +68,9 @@ Definition graph_rep (g: graph) : mpred :=
 
 (** An inductive predicate stating that a tree is present in a graph.
     Note that this is a purely propositional predicate.
- *) 
+ *)
 Inductive tree_in_graph (g: graph) : tree -> val -> Prop :=
-| TIG_E: tree_in_graph g E nullval (** The empty tree corresponds to the null value. *) 
+| TIG_E: tree_in_graph g E nullval (** The empty tree corresponds to the null value. *)
 | TIG_T: (** Definition of a leaf *)
     forall (p : val) (n : int) tl (pl : val) tr (pr: val),
     In (p, (Vint n, (pl, pr))) g ->
@@ -79,10 +78,10 @@ Inductive tree_in_graph (g: graph) : tree -> val -> Prop :=
     tree_in_graph g tr pr ->
     tree_in_graph g (T n tl tr) p.
 
-(** The VST specification of [sum] contains of a spatial and a propositional part: 
+(** The VST specification of [sum] contains of a spatial and a propositional part:
  - In the spatial part, we declare the spatial graph representation of [g].
  - In the propositional part, we state that graph [g] contains a representation of tree [t] at position [p].
-*) 
+*)
 Definition sum_spec :=
  DECLARE _sum
  WITH g: graph, t: tree, p: val
@@ -95,67 +94,67 @@ Definition sum_spec :=
     LOCAL(temp ret_temp (Vint (sum t)))
     SEP (graph_rep g).
 
-Definition Gprog : funspecs := [ sum_spec ]. 
+Definition Gprog : funspecs := [ sum_spec ].
 
-(** We require several intermediate facts, which will later be provided automatically by the CertiGraph library. *)  
+(** We require several intermediate facts, which will later be provided automatically by the CertiGraph library. *)
 
-(** Predicate needed for the localization *) 
-Lemma graph_rep_In (g : graph) (n: reptype t_struct_tree) p: 
-  In (p, n) g -> graph_rep g = (data_at Ews t_struct_tree n p * (data_at Ews t_struct_tree n p -* graph_rep g))%logic. 
+(** Predicate needed for the localization *)
+Lemma graph_rep_In (g : graph) (n: reptype t_struct_tree) p:
+  In (p, n) g -> graph_rep g = (data_at Ews t_struct_tree n p * (data_at Ews t_struct_tree n p -* graph_rep g))%logic.
 Proof.
-  intros. apply pred_ext. 
-  - induction g; simpl in *. 
-    + inversion H. 
+  intros. apply pred_ext.
+  - induction g; simpl in *.
+    + inversion H.
     + destruct H as [|]; subst.
-      * simpl. entailer!. apply wand_sepcon_adjoint. entailer!. 
+      * simpl. entailer!. apply wand_sepcon_adjoint. entailer!.
       * specialize (IHg H). sep_apply IHg. entailer. cancel.
         rewrite <- wand_sepcon_adjoint.
-        cancel. rewrite sepcon_comm. apply modus_ponens_wand. 
+        cancel. rewrite sepcon_comm. apply modus_ponens_wand.
   - sep_apply modus_ponens_wand. entailer.
 Qed.
 
 (** We will require local facts for  [tree_in_graph]. *)
 
-Lemma graph_rep_In_valid p v g: 
-  In (p, v) g -> graph_rep g |-- valid_pointer p. 
+Lemma graph_rep_In_valid p v g:
+  In (p, v) g -> graph_rep g |-- valid_pointer p.
 Proof.
   intros H. rewrite (graph_rep_In _ _ _ H). entailer!.
 Qed.
- 
-Lemma valid_pointer_tree g t p: 
-tree_in_graph g t p -> graph_rep g |-- valid_pointer p. 
-Proof. 
-  induction 1. 
-  - entailer!. 
+
+Lemma valid_pointer_tree g t p:
+tree_in_graph g t p -> graph_rep g |-- valid_pointer p.
+Proof.
+  induction 1.
+  - entailer!.
   - entailer!. eauto using graph_rep_In_valid.
 Qed.
 
-Hint Resolve valid_pointer_tree : valid_pointer.
+#[local] Hint Resolve valid_pointer_tree : valid_pointer.
 
-Lemma graph_rep_local_facts p v g: 
-  In (p, v) g -> graph_rep g |-- !!(isptr p). 
+Lemma graph_rep_local_facts p v g:
+  In (p, v) g -> graph_rep g |-- !!(isptr p).
 Proof.
   intros H. rewrite (graph_rep_In _ _ _ H). entailer!.
 Qed.
 
-Lemma treerep_local_facts g: 
-graph_rep g |-- !!(forall t p, tree_in_graph g t p ->  is_pointer_or_null p). 
+Lemma treerep_local_facts g:
+graph_rep g |-- !!(forall t p, tree_in_graph g t p ->  is_pointer_or_null p).
 Proof.
   rewrite prop_forall. apply allp_right. intros t.
-  rewrite prop_forall. apply allp_right. intros v. 
+  rewrite prop_forall. apply allp_right. intros v.
   rewrite prop_impl. apply imp_andp_adjoint. entailer.
   induction H.
    - entailer!.
-   - entailer. sep_apply (graph_rep_local_facts p (Vint n, (pl, pr))). entailer!. 
+   - entailer. sep_apply (graph_rep_local_facts p (Vint n, (pl, pr))). entailer!.
 Qed.
 
-Hint Resolve treerep_local_facts : saturate_local.
+#[local] Hint Resolve treerep_local_facts : saturate_local.
 
 (** Inversion predicates for tree representations *)
 Lemma tree_in_graph_null g t:
-  tree_in_graph g t nullval -> graph_rep g |-- !!(t = E). 
+  tree_in_graph g t nullval -> graph_rep g |-- !!(t = E).
 Proof.
-  intros H. 
+  intros H.
   inversion H; subst.
   - entailer!.
   - sep_apply (graph_rep_In _ _ _ H0). entailer!.
@@ -165,50 +164,50 @@ Lemma tree_in_graph_nonnull: forall g t p,
   p <> nullval -> tree_in_graph g t p ->
   graph_rep g |--
     EX pl pr: val, EX n : int, EX tl tr : tree,
-      graph_rep g && !! (In (p, (Vint n, (pl, pr))) g /\ t = T n tl tr /\ tree_in_graph g tl pl /\ tree_in_graph g tr pr). 
+      graph_rep g && !! (In (p, (Vint n, (pl, pr))) g /\ t = T n tl tr /\ tree_in_graph g tl pl /\ tree_in_graph g tr pr).
 Proof.
-  intros. inversion H0; subst. 
-  - congruence. 
-  - Exists pl pr n tl tr. entailer!. 
+  intros. inversion H0; subst.
+  - congruence.
+  - Exists pl pr n tl tr. entailer!.
 Qed.
 
 
-(** *** The main theorem *) 
+(** *** The main theorem *)
 Lemma body_sum: semax_body Vprog Gprog f_sum sum_spec.
 Proof.
   start_function.
-  forward_if. 
+  forward_if.
   { sep_apply (valid_pointer_tree _ _ _ H). entailer!. }
-  - subst. sep_apply (tree_in_graph_null _ _ H). 
+  - subst. sep_apply (tree_in_graph_null _ _ H).
     forward.
-  - sep_apply (tree_in_graph_nonnull _ _ _ H0 H).  
-    Intros pl pr n tl tr. subst. 
+  - sep_apply (tree_in_graph_nonnull _ _ _ H0 H).
+    Intros pl pr n tl tr. subst.
 
     assert_PROP (is_pointer_or_null pl). { entailer!. eauto. }
     assert_PROP (is_pointer_or_null pr). { entailer!. eauto. }
-    
-    (** Here, the localization tactic is used to single out the representation of one node. *)                                    
+
+    (** Here, the localization tactic is used to single out the representation of one node. *)
     localize [data_at Ews t_struct_tree (Vint n, (pl, pr)) p].
-    (* unfold abbreviate in RamL. 
+    (* unfold abbreviate in RamL.
     unfold abbreviate in RamG. *)
     forward.
-    (** We can undo the localization. *) 
+    (** We can undo the localization. *)
     unlocalize [graph_rep g].
-    { rewrite <- graph_rep_In; auto. } 
+    { rewrite <- graph_rep_In; auto. }
 
-    forward_call (g, tl, pl). 
+    forward_call (g, tl, pl).
 
-    localize [data_at Ews t_struct_tree (Vint n, (pl, pr)) p]. 
+    localize [data_at Ews t_struct_tree (Vint n, (pl, pr)) p].
     forward.
     unlocalize [graph_rep g].
-    { rewrite <- graph_rep_In; auto. } 
+    { rewrite <- graph_rep_In; auto. }
 
-    forward_call (g, tr, pr). 
+    forward_call (g, tr, pr).
 
-    localize [data_at Ews t_struct_tree (Vint n, (pl, pr)) p]. 
+    localize [data_at Ews t_struct_tree (Vint n, (pl, pr)) p].
     forward.
     unlocalize [graph_rep g].
-    { rewrite <- graph_rep_In; auto. } 
+    { rewrite <- graph_rep_In; auto. }
 
     forward. entailer!.
     now rewrite Int.add_assoc.
@@ -216,49 +215,228 @@ Qed.
 
 End SimplifiedModel.
 
+(** ** Part 2: In CertiGraph *)
 
+Require Import CertiGraph.graph.graph_model.
+Require Import CertiGraph.graph.path_lemmas.
+Require Import CertiGraph.msl_application.Graph.
 
-(** ** Part 2: In CertiGraph *) 
+Section CertiGraphModel.
 
-Require Import CertiGraph. (* TODO *) 
+(* With the help of the CertiGraph library, we can treat the data in
+   the heap as a graph and reason about it. *)
 
-Definition graph : Type := (* TODO *).
+(* Every graph must have a type called PreGraph. *)
+
+Print PreGraph.
+
+(* To declare a PreGraph, we need to provide the types of the vertices
+   and edges, also with the proofs which say their equliaties are
+   decidable.
+
+   In our case, we can simply define val in VST as the vertex
+   type. The definition of the edge type could be (val * LR) where LR
+   is an inductive type indicating left or right, because what we have
+   is a binary tree here. *)
+
+Definition VType : Type := val.
+
+Inductive LR := L | R.
+
+Definition EType : Type := val * LR.
+
+#[local] Instance V_EqDec: EquivDec.EqDec VType eq.
+Proof. repeat intro. apply Val.eq. Defined.
+
+#[local] Instance E_EqDec: EquivDec.EqDec EType eq.
+Proof.
+  intros [x lx] [y ly]. destruct (Val.eq x y).
+  - subst. destruct lx, ly; [left | right ..| left]; easy.
+  - right. destruct lx, ly; congruence.
+Defined.
+
+(* V_EqDec and E_EqDec would be maximally inserted. *)
+
+Check (PreGraph VType EType).
+
+(* When we declared a type like above, we assume we have all the four
+   components of PreGraph: two predicates (vvalid and evalid) and two
+   functions (src and dst). Please refer to the section 4.1 in [1] for
+   more information. *)
+
+(* PreGraph just describes the topological layout of a graph. The
+   graph used in concrete programs usually carry more information. The
+   CertiGraph library provides LabeledGraph, which allows us to
+   represent any type of "labels" attached to vertices or/and edges,
+   or even the whole graph. *)
+
+(* In this case, each node carries an unsigned integer which can be
+   represented by type int. We specify the unit type for labels of edges
+   and the whole graph. *)
+
+Definition graph: Type := (LabeledGraph VType EType int unit unit).
+
+(* Even after defining the LabeledGraph, there are still too many
+   possibilities for our graphs. The graph in our case is very
+   special: it is a binary tree. So we can define a predicate to show
+   this: *)
+
+Local Coercion pg_lg: LabeledGraph >-> PreGraph.
 
 Inductive tree_in_graph (g: graph) : tree -> val -> Prop :=
-| TIG_E: tree_in_graph g E nullval (** The empty tree corresponds to the null value. *) 
+| TIG_E: tree_in_graph g E nullval (** The empty tree corresponds to the null value. *)
 | TIG_T: (** Definition of a leaf *)
-    forall (p : val) (n : int) tl (pl : val) tr (pr: val),
-(*     graph_has_v (p, (Vint n, (pl, pr))) g ->
-       replace with a suitable predicate.
- *)
-    tree_in_graph g tl pl ->
-    tree_in_graph g tr pr ->
-    tree_in_graph g (T n tl tr) p.
+  forall (p : val) tl tr,
+    vvalid g p ->
+    tree_in_graph g tl (dst g (p, L)) ->
+    tree_in_graph g tr (dst g (p, R)) ->
+    tree_in_graph g (T (vlabel g p) tl tr) p.
 
+(* So far, all these definitions are pure mathematical. The next step
+   is connecting the pure mathematical graph and its spatial
+   representation. The CertiGraph library provides some helper
+   definitions for such connections. All we need to do is to
+   implementing some classes. *)
 
-(** An inductive predicate corresponding to ... *) 
+(* This is just a wrapper for the decidable equality of vertices and edges *)
+
+#[local] Instance PGBA_VST: PointwiseGraphBasicAssum val (val * LR).
+Proof. constructor; apply _. Defined.
+
+(* The following two classes together form the spatial representation
+   of a single vertex, the first maps a vertex to a intermediate type,
+   the second maps the intermediate value to the spatial predicate. *)
+
+#[local] Instance PGC_VST: PointwiseGraphConstructor val (val * LR) int unit unit (int * val * val) unit.
+Proof. constructor. exact (fun g v => (vlabel g v, dst g (v, L), dst g (v, R))). exact (fun _ _ => tt). Defined.
+
+#[local] Instance PGP_VST: PointwiseGraphPred VType EType (int * val * val) unit mpred.
+Proof.
+  constructor. exact (fun p dlr => match dlr with | (d, l, r) => data_at Ews t_struct_tree (Vint d, (l, r)) p end).
+  exact (fun _ _ => emp).
+Defined.
+
+(* This is just a wrapper for various VST classes *)
+
+#[local] Instance PGA_VST: PointwiseGraphAssum PGP_VST.
+Proof. refine (Build_PointwiseGraphAssum _ _ _ _ _ _ _ _ _ _ _). Defined.
+
+(* Now we can define the spatial representation of our
+   graph. Basically it iteratively separates all valid vertex
+   representations. *)
+
+Definition graph_rep (g: graph) := full_vertices_at g.
+
+(* The following 4 lines coerce the type graph to the type
+   PointwiseGraph, so that we can use terms like "vgamma g p" without
+   writing conversion function explicitly. *)
+
+Definition SGraph := PointwiseGraph val (val * LR) (int * val * val) unit.
+Definition graph_SGraph (G: graph): SGraph := Graph_PointwiseGraph G.
+Local Coercion graph_SGraph: graph >-> SGraph.
+Local Identity Coercion SGraph_PointwiseGraph: SGraph >-> PointwiseGraph.
 
 Definition sum_spec :=
  DECLARE _sum
- WITH g: graph, t: tree, p: val, sh: wshare, x : addr
+ WITH g: graph, t: tree, p: val
   PRE  [ tptr t_struct_tree ]
        PROP(tree_in_graph g t p)
        PARAMS (p)
-       SEP (graph_rep sh x g)
-       (* The term "g" has type "graph" while it is expected to have type "LabeledGraph addr (addr * LR) bool unit unit". *) 
+       SEP (graph_rep g)
   POST [ tuint ]
     PROP()
     LOCAL(temp ret_temp (Vint (sum t)))
     SEP (graph_rep g).
 
+Definition Gprog : funspecs := [ sum_spec ].
+
+(* Here we use the lemma vertices_at_ramif_1_stable the CertiGraph
+   library to establish graph_rep_In. *)
+
+Lemma graph_rep_In (g : graph) p:
+  vvalid g p -> graph_rep g = (vertex_at p (vgamma g p) * (vertex_at p (vgamma g p) -* graph_rep g))%logic.
+Proof.
+  intros. apply pred_ext.
+  - apply (@vertices_at_ramif_1_stable _ _ _ _ PGBA_VST mpred PGP_VST PGA_VST); auto.
+  - sep_apply modus_ponens_wand. entailer.
+Qed.
+
+(* The rest proofs are almost the same. *)
+
+Lemma valid_pointer_tree g t p:
+  tree_in_graph g t p -> graph_rep g |-- valid_pointer p.
+Proof.
+  intros. inversion H; subst.
+  - entailer !.
+  - rewrite (graph_rep_In g p); auto. simpl vertex_at. entailer !.
+Qed.
+
+#[local] Hint Resolve valid_pointer_tree : valid_pointer.
+
+Lemma treerep_local_facts g:
+  graph_rep g |-- !!(forall t p, tree_in_graph g t p ->  is_pointer_or_null p).
+Proof.
+  do 2 (rewrite prop_forall; apply allp_right; intros).
+  rewrite prop_impl. apply imp_andp_adjoint. entailer.
+  inversion H.
+  - entailer!.
+  - entailer. rewrite (graph_rep_In _ _ H0). simpl vertex_at. entailer!.
+Qed.
+
+#[local] Hint Resolve treerep_local_facts : saturate_local.
+
+Lemma tree_in_graph_null g t:
+  tree_in_graph g t nullval -> graph_rep g |-- !!(t = E).
+Proof.
+  intros H.
+  inversion H; subst.
+  - entailer!.
+  - sep_apply (graph_rep_In _ _ H0). simpl vertex_at. entailer !.
+Qed.
 
 Lemma body_sum: semax_body Vprog Gprog f_sum sum_spec.
 Proof.
- (* TODO *) 
-Admitted.
+  start_function.
+  forward_if.
+  { sep_apply (valid_pointer_tree _ _ _ H). entailer !. }
+  - subst. sep_apply (tree_in_graph_null _ _ H). forward.
+  - inversion H; subst. 1: now exfalso.
+    assert_PROP (is_pointer_or_null (dst g (p, L))). { entailer!. eauto. }
+    assert_PROP (is_pointer_or_null (dst g (p, R))). { entailer!. eauto. }
+
+    (** Here, the localization tactic is used to single out the representation of one node. *)
+    localize [vertex_at p (vgamma g p)].
+    simpl vertex_at.
+    forward.
+    (** We can undo the localization. *)
+    unlocalize [graph_rep g].
+    { rewrite <- graph_rep_In; auto. }
+
+    forward_call (g, tl, (dst g (p, L))).
+
+    localize [vertex_at p (vgamma g p)].
+    simpl vertex_at.
+    forward.
+    unlocalize [graph_rep g].
+    { rewrite <- graph_rep_In; auto. }
+
+    forward_call (g, tr, (dst g (p, R))).
+
+    localize [vertex_at p (vgamma g p)].
+    simpl vertex_at.
+    forward.
+    unlocalize [graph_rep g].
+    { rewrite <- graph_rep_In; auto. }
+
+    forward. entailer!.
+    now rewrite Int.add_assoc.
+Qed.
+
+End CertiGraphModel.
 
 
-(** Related Work: 
+(** Related Work:
 
+[1] Certifying Graph-Manipulating C Programs via Localizations within Data Structures (OOPSLA 2019)
 
-*) 
+*)
